src/go_lang/examples/goose_unittest.v
@@ -72,6 +72,11 @@ Definition useSliceIndexing: val :=
     let: "x" := SliceGet "s" #0 in
     "x".
 
+Definition useSlice2: val :=
+  λ: <>,
+    let: "s" := NewSlice byteT #1 in
+    "s".
+
 Definition useMap: val :=
   λ: <>,
     let: "m" := NewMap (slice.T byteT) in
@@ -610,3 +615,21 @@ Definition testStore: val :=
     let: "x" := zero_val uint64T in
     "x" <- #3;;
     !"x".
+
+Definition testLongSlice: val :=
+  λ: <>,
+     let: "x" := #72 in
+     let: "e" := NewSlice byteT #8 in
+     "e".
+
+Definition testUInt64EncDec: val :=
+  λ: "x",
+     let: "r" := NewSlice byteT #8 in
+     let: "e" := struct.new Enc.S [
+                             "p" ::= "r"
+                           ] in
+     let: "d" := struct.new Dec.S [
+                              "p" ::= "r"
+                            ] in
+     Enc__UInt64 "e" "x";;
+     Dec__UInt64 "d".
